update

theory/Semantics.thy
@@ -163,4 +163,7 @@ abbreviation concur_steps :: "state_pool \<Rightarrow> state_pool \<Rightarrow> 
   "\<E> \<rightarrow>* \<E>' \<equiv> star concur_step \<E> \<E>'"
 
 
+fun start_state :: "exp \<Rightarrow> state_pool" where
+ "start_state e = [[] \<mapsto> \<langle>e;Map.empty;[]\<rangle>]"
+
 end
